#+title: Lösungen zum 4. Übungsblatt
#+date: 2018-11-05
#+email: tobias.denkinger@tu-dresden.de
#+options: toc:nil

* Lösungen zu Aufgabe 1 (AGS 2.2.39)
** Teilaufgabe a

#+begin_src elisp
f(ρ) = S⎛⟦[B]b⟧(ρ)⎞ = ⎛ρ(B) ⋅ {b} ∪ {b}⎞
       B⎝⟦Sb⟧(ρ)  ⎠   ⎝ρ(S) ⋅ {b}      ⎠

⊥ = S⎛∅⎞
    B⎝∅⎠
  ↦ ⎛{b}⎞
    ⎝ ∅ ⎠
  ↦ ⎛{b} ⎞
    ⎝{b²}⎠
  ↦ ⎛{b, b³}⎞
    ⎝{b²}   ⎠
  ↦ ⎛{b, b³} ⎞
    ⎝{b², b⁴}⎠
  ↦ ⎛{b, b³, b⁵}⎞
    ⎝{b², b⁴}   ⎠
#+end_src

** Teilaufgabe b

  * W(ℰ, S) = {b²ⁿ⁺¹ ∣ n ∈ ℕ}
  * W(ℰ, B) = {b²ⁿ ∣ n ∈ ℕ₊}

** Teilaufgabe c

#+begin_src elisp
Seien ρ(S) = ρ(A) = {(ba)ⁿb ∣ n ∈ ℕ}.  Zu zeigen: ⟦{ba}A⟧(ρ) = ρ(S).

Beweis:

⟦{ba}A⟧(ρ)
= ⟦{ba}⟧(ρ) ⋅ ⟦A⟧(ρ)
= (⟦ba⟧(ρ))* ⋅ ⟦A⟧(ρ)
= (⟦b⟧(ρ) ⋅ ⟦a⟧(ρ))* ⋅ ⟦A⟧(ρ)
= ({b} ⋅ {a})* ⋅ ⟦A⟧(ρ)
= ({b} ⋅ {a})* ⋅ ρ(A)
= ({b} ⋅ {a})* ⋅ {(ba)ⁿb ∣ n ∈ ℕ}
= {ba}* ⋅ {(ba)ⁿb ∣ n ∈ ℕ}
= {(ba)ᵐ ∣ m ∈ ℕ} ⋅ {(ba)ⁿb ∣ n ∈ ℕ}
= {(ba)ᵐ(ba)ⁿb ∣ m, n ∈ ℕ}
= {(ba)ᵏb ∣ m, n ∈ ℕ, k = m + n}
= {(ba)ᵏb ∣ k ∈ ℕ}
= {(ba)ⁿb ∣ n ∈ ℕ}
= ρ(S)
#+end_src

* Lösungen zu Aufgabe 2 (AGS 3.1.2)

** Teilaufgabe a

#+include: "sol04-2a.c" src c

** Teilaufgabe b

#+include: "sol04-2b.c" src c

** Teilaufgabe a

#+include: "sol04-2c.c" src c

* Lösungen zu Aufgabe 3 (AGS 3.1.6)

/Hausaufgabe/
